src/Std/Tactic/BVDecide/LRAT/Internal/Formula/RupAddResult.lean
@@ -118,8 +118,8 @@ theorem insertUnitInvariant_insertUnit {n : Nat} (assignments0 : Array Assignmen
           · rw [Array.getElem_modify_self]
             simp only [← i_eq_l, h1]
           · constructor
-            · simp only [getElem!, l_in_bounds, ↓reduceDIte, Array.get_eq_getElem,
-                Bool.not_eq_true, decidableGetElem?] at h3
+            · simp only [getElem!_def, l_in_bounds, Array.getElem?_eq_getElem,
+                Bool.not_eq_true] at h3
               simp only [← i_eq_l, ← h1]
               simp only [i_eq_l, h3]
             · intro k hk
@@ -183,7 +183,7 @@ theorem insertUnitInvariant_insertUnit {n : Nat} (assignments0 : Array Assignmen
         | true, true =>
           exfalso
           have assignments_i_rw : assignments[i.1]! = assignments[i.1] := by
-            simp only [getElem!, i_in_bounds, ↓reduceDIte, Array.get_eq_getElem, decidableGetElem?]
+            simp only [getElem!_def, i_in_bounds, Array.getElem?_eq_getElem]
           rw [hl, ← i_eq_l, assignments_i_rw, h2] at h5
           exact h5 (has_add _ true)
         | true, false =>
@@ -206,7 +206,7 @@ theorem insertUnitInvariant_insertUnit {n : Nat} (assignments0 : Array Assignmen
                   | neg =>
                     simp only [addAssignment, addPosAssignment, h, ite_true] at h2
                     simp only [i_eq_l] at h2
-                    simp [hasAssignment, hl, getElem!, l_in_bounds, h2, hasNegAssignment, decidableGetElem?] at h5
+                    simp [hasAssignment, hl, getElem!_def, l_in_bounds, h2, hasNegAssignment] at h5
                   | both => simp +decide only [h] at h3
                 · intro k k_ne_j k_ne_l
                   rw [Array.getElem_push]
@@ -242,7 +242,7 @@ theorem insertUnitInvariant_insertUnit {n : Nat} (assignments0 : Array Assignmen
                   | pos =>
                     simp only [addAssignment, h, ite_false, addNegAssignment, reduceCtorEq] at h2
                     simp only [i_eq_l] at h2
-                    simp [hasAssignment, hl, getElem!, l_in_bounds, h2, hasPosAssignment, decidableGetElem?] at h5
+                    simp [hasAssignment, hl, getElem!_def, l_in_bounds, h2, hasPosAssignment] at h5
                   | neg  => simp +decide only [h] at h3
                   | both => simp +decide only [h] at h3
                 · intro k k_ne_l k_ne_j
@@ -263,7 +263,7 @@ theorem insertUnitInvariant_insertUnit {n : Nat} (assignments0 : Array Assignmen
         | false, false =>
           exfalso
           have assignments_i_rw : assignments[i.1]! = assignments[i.1] := by
-            simp [getElem!, i_in_bounds, decidableGetElem?]
+            simp [getElem!_def, i_in_bounds]
           rw [hl, ← i_eq_l, assignments_i_rw, h2] at h5
           exact h5 (has_add _ false)
       · next i_ne_l =>
@@ -355,7 +355,7 @@ theorem insertUnitInvariant_insertUnit {n : Nat} (assignments0 : Array Assignmen
                   · exact k_eq_units_size
                 simp only [k_eq_units_size, Array.getElem_push_eq, ne_eq]
                 intro l_eq_i
-                simp [getElem!, l_eq_i, i_in_bounds, h3, has_both, decidableGetElem?] at h
+                simp [getElem!_def, l_eq_i, i_in_bounds, h3, has_both] at h
 
 theorem insertUnitInvariant_insertUnit_fold {n : Nat} (assignments0 : Array Assignment)
     (assignments0_size : assignments0.size = n) (rupUnits : Array (Literal (PosFin n)))
@@ -791,8 +791,7 @@ theorem confirmRupHint_preserves_invariant_helper {n : Nat} (f : DefaultFormula 
         · simp only [l_eq_i, Array.getElem_modify_self, List.get, h1]
         · constructor
           · simp only [List.get, Bool.not_eq_true]
-            simp only [getElem!, l_in_bounds, ↓reduceDIte, Array.get_eq_getElem,
-              Bool.not_eq_true, decidableGetElem?] at h
+            simp only [getElem!_def, l_in_bounds, Array.getElem?_eq_getElem, Bool.not_eq_true] at h
             simp only [l_eq_i, h1] at h
             exact h
           · intro k k_ne_zero
@@ -840,7 +839,7 @@ theorem confirmRupHint_preserves_invariant_helper {n : Nat} (f : DefaultFormula 
         intro l_eq_l'
         rw [l_eq_i] at h
         simp only [l'] at l_eq_l'
-        simp [getElem!, i_in_bounds, h1, l_eq_l', has_add, decidableGetElem?] at h
+        simp [getElem!_def, i_in_bounds, h1, l_eq_l', has_add] at h
       by_cases l.2
       · next l_eq_true =>
         rw [l_eq_true] at l_ne_l'
@@ -863,9 +862,9 @@ theorem confirmRupHint_preserves_invariant_helper {n : Nat} (f : DefaultFormula 
             · constructor
               · simp only [l'] at l'_eq_false
                 simp only [l'_eq_false, hasAssignment, ite_false] at h2
-                simp only [hasAssignment, l_eq_true, getElem!, l_eq_i, i_in_bounds,
-                  Array.get_eq_getElem, ↓reduceIte, ↓reduceDIte, h1, addAssignment, l'_eq_false,
-                  hasPos_addNeg, decidableGetElem?, reduceCtorEq] at h
+                simp only [hasAssignment, l_eq_true, ↓reduceIte, l_eq_i, getElem!_def, i_in_bounds,
+                  Array.getElem?_eq_getElem, h1, addAssignment, l'_eq_false, reduceCtorEq,
+                  hasPos_addNeg, l'] at h
                 exact unassigned_of_has_neither _ h h2
               · intro k k_ne_zero k_ne_j_succ
                 have k_eq_succ : ∃ k' : Nat, ∃ k'_succ_in_bounds : k' + 1 < (l :: acc.2.1).length, k = ⟨k' + 1, k'_succ_in_bounds⟩ := by
@@ -912,8 +911,9 @@ theorem confirmRupHint_preserves_invariant_helper {n : Nat} (f : DefaultFormula 
             · constructor
               · simp only [l'] at l'_eq_true
                 simp only [hasAssignment, l'_eq_true, ite_true] at h2
-                simp only [hasAssignment, l_eq_false, ↓reduceIte, ↓reduceDIte, getElem!, l_eq_i, i_in_bounds,
-                  Array.get_eq_getElem, h1, addAssignment, l'_eq_true, hasNeg_addPos, decidableGetElem?, reduceCtorEq] at h
+                simp only [hasAssignment, l_eq_false, reduceCtorEq, ↓reduceIte, l_eq_i,
+                  getElem!_def, i_in_bounds, Array.getElem?_eq_getElem, h1, addAssignment,
+                  l'_eq_true, hasNeg_addPos, l'] at h
                 exact unassigned_of_has_neither _ h2 h
               · intro k k_ne_j_succ k_ne_zero
                 have k_eq_succ : ∃ k' : Nat, ∃ k'_succ_in_bounds : k' + 1 < (l :: acc.2.1).length, k = ⟨k' + 1, k'_succ_in_bounds⟩ := by
@@ -992,7 +992,7 @@ theorem confirmRupHint_preserves_invariant_helper {n : Nat} (f : DefaultFormula 
       simp only [hasAssignment, Bool.not_eq_true] at h
       split at h
       all_goals
-        simp +decide [getElem!, l_eq_i, i_in_bounds, h1, decidableGetElem?] at h
+        simp +decide [getElem!_def, l_eq_i, i_in_bounds, h1] at h
     constructor
     · rw [Array.getElem_modify_of_ne l_ne_i]
       exact h1
